AutoKchp/RadixSort.lean
@@ -1,82 +1,11 @@
-import Automata.Counting
+module
+
+import AutoKchp.Counting
+import AutoKchp.Util
 
 /-
 Counting sort table construction
 -/
-
-def Vector.modify {α} {k: Nat} (v: Vector α k) (i: Fin k) (f: α → α): Vector α k :=
-  ⟨v.toArray.modify i.val f, Eq.trans Array.size_modify v.size_toArray⟩
-
-
-theorem Vector.get_modify_self {α} {k: Nat} {v: Vector α k} {i: Fin k} {f: α → α}:
-    (v.modify i f).get i = f (v.get i) :=
-  Array.getElem_modify_self f ((v.modify i f).size_toArray.symm ▸ i.isLt)
-
-
-theorem Vector.get_modify_of_ne {α} {k: Nat} {v: Vector α k} {i j: Fin k} {f: α → α} (h: i ≠ j):
-    (v.modify i f).get j = v.get j :=
-  Array.getElem_modify_of_ne (Fin.val_ne_iff.mpr h) f ((v.modify i f).size_toArray.symm ▸ j.isLt)
-
-
-theorem Vector.get_ext {α} {k: Nat} {v w: Vector α k} (h: ∀ i: Fin k, v.get i = w.get i): v = w :=
-  Vector.ext (fun i hi => h ⟨i, hi⟩)
-
-
-theorem Vector.get_replicate {α} {k: Nat} {a: α} {i: Fin k}: (Vector.replicate k a).get i = a :=
-  have lt: i.val < (Vector.replicate k a).toArray.size :=
-    ((Vector.replicate k a).size_toArray.symm) ▸ i.isLt
-  Array.getElem_replicate lt
-
-
-theorem Vector.modify_modify_self {α} {k: Nat} {v: Vector α k} {i: Fin k} {f g: α → α}:
-    (v.modify i f).modify i g = v.modify i (g ∘ f) :=
-  Vector.get_ext (fun j =>
-    if eq: i = j then
-        eq.symm ▸
-        Vector.get_modify_self.symm ▸
-        Vector.get_modify_self.symm ▸
-        Vector.get_modify_self.symm ▸ rfl
-    else
-        (Vector.get_modify_of_ne eq).symm ▸
-        (Vector.get_modify_of_ne eq).symm ▸
-        (Vector.get_modify_of_ne eq).symm ▸ rfl
-  )
-
-
-theorem Vector.modify_modify_of_ne {α} {k: Nat} {v: Vector α k} {i j: Fin k} {f g: α → α} (h: i ≠ j):
-    (v.modify i f).modify j g = (v.modify j g).modify i f :=
-  Vector.get_ext (fun a =>
-    if eqi: i = a then
-      eqi ▸
-      (Vector.get_modify_of_ne h.symm).symm ▸
-      Vector.get_modify_self.symm ▸
-      Vector.get_modify_self.symm ▸
-      (Vector.get_modify_of_ne h.symm).symm ▸ rfl
-    else if eqj: j = a then
-      eqj ▸
-      (Vector.get_modify_of_ne h).symm ▸
-      Vector.get_modify_self.symm ▸
-      Vector.get_modify_self.symm ▸
-      (Vector.get_modify_of_ne h).symm ▸ rfl
-    else
-      (Vector.get_modify_of_ne eqi).symm ▸
-      (Vector.get_modify_of_ne eqj).symm ▸
-      (Vector.get_modify_of_ne eqj).symm ▸
-      (Vector.get_modify_of_ne eqi).symm ▸ rfl
-  )
-
-
-theorem Vector.modify_comm {α} {k: Nat} {v: Vector α k} {i j: Fin k}
-  {f: α → α} {g: α → α} (h: g ∘ f = f ∘ g):
-    (v.modify i f).modify j g = (v.modify j g).modify i f :=
-  if eq: i = j then
-    eq ▸
-    Vector.modify_modify_self.symm ▸
-    Vector.modify_modify_self.symm ▸
-    (congrArg _ h)
-  else
-    Vector.modify_modify_of_ne eq
-
 
 def addToTable {k: Nat} (f: Nat → Fin k) (v: Vector (List Nat) k): Nat → Vector (List Nat) k
   | 0 => v
@@ -183,15 +112,6 @@ theorem constructTable'_mem_iff {k: Nat} {f: Nat → Fin k} {i: Fin k} {p q: Nat
 
 
 --Injectivity
-theorem List.nodup_singleton {α} {a: α}: [a].Nodup :=
-  List.nodup_cons.mpr ⟨List.not_mem_nil, List.nodup_nil⟩
-
-
-theorem List.nodup_append_singleton {α} {l: List α} {a: α} (h1: a ∉ l) (h2: l.Nodup):
-    (l ++ [a]).Nodup :=
-  List.nodup_append.mpr ⟨h2, List.nodup_singleton,
-    fun _ hx _ hy hxy => h1 ((hxy ▸ (List.mem_singleton.mp hy)) ▸ hx)⟩
-
 
 theorem constructTable'_nodup {k: Nat} {f: Nat → Fin k} {i: Fin k}:
     {n: Nat} → ((constructTable' f n).get i).Nodup
@@ -245,46 +165,6 @@ theorem constructTable_stable_of_lt {k: Nat} {f: Nat → Fin k} {p q n: Nat}
 Counting sort
 -/
 
-theorem List.flatten_append_eq_foldl_append {α} {u: List α}:
-    {l: List (List α)} → u ++ l.flatten = l.foldl (fun acc v => acc ++ v) u
-  | [] => List.flatten_nil ▸ List.append_nil _ ▸ List.foldl_nil ▸ rfl
-  | _::_ => List.flatten_cons.symm ▸ (List.append_assoc _ _ _ ▸ List.flatten_append_eq_foldl_append)
-
-
-theorem List.flatten_eq_foldl_append {α} {l: List (List α)}:
-    l.flatten = l.foldl (fun acc u => acc ++ u) [] :=
-  List.flatten_append_eq_foldl_append ▸ List.nil_append _
-
-
-theorem List.concat_eq_foldl {α} {u: List α}:
-    {v: List α} → u ++ v = v.foldl (fun acc a => acc ++ [a]) u
-  | [] => (List.append_nil _).symm ▸ (List.foldl_nil ▸ rfl)
-  | _::_ => List.foldl_cons.symm ▸ List.concat_eq_foldl ▸ (List.append_cons u _ _) ▸ rfl
-
-
-theorem List.flatten_eq_foldl_foldl {α} {l: List (List α)}:
-    l.flatten = l.foldl (fun acc u => u.foldl (fun acc a => acc ++ [a]) acc) [] :=
-  List.flatten_eq_foldl_append ▸ congrArg
-    (fun x => l.foldl x [])
-    (funext (fun _ => funext (fun _ => List.concat_eq_foldl)))
-
-
-def Array.flattenLists {α} {v: Array (List α)}: Array α :=
-  v.foldl (fun acc l => l.foldl (fun acc a => acc.push a) acc) Array.empty
-
-
-theorem Array.toList_flattenLists {α} {v: Array (List α)}:
-    v.flattenLists.toList = v.foldl (fun acc l => l.foldl (fun acc a => acc ++ [a]) acc) [] :=
-  (Array.foldl_hom Array.toList fun _ _ => (
-    List.foldl_hom Array.toList fun _ _ => Eq.symm toList_push
-  )).symm
-
-
-theorem Array.toList_flattenLists_eq_flatten_toList {α} {v: Array (List α)}:
-    v.flattenLists.toList = v.toList.flatten :=
-  Eq.trans ((Array.foldl_toList _) ▸ Array.toList_flattenLists) List.flatten_eq_foldl_foldl.symm
-
-
 def countingSort {k: Nat} (f: Nat → Fin k) (n: Nat): Array Nat :=
   (constructTable f n).toArray.flattenLists
 
@@ -300,9 +180,6 @@ theorem countingSort_eq_countingSort' {k: Nat} {f: Nat → Fin k} {n: Nat}:
 
 
 --Surjectivity
-theorem Vector.get_mem {α} {k: Nat} {v: Vector α k} {i: Fin k}: v.get i ∈ v :=
-    Vector.getElem_mem i.isLt
-
 
 theorem countingSort'_mem_of_lt {k: Nat} {f: Nat → Fin k} {p q: Nat} (h: p < q):
     p ∈ countingSort' f q :=
@@ -311,11 +188,6 @@ theorem countingSort'_mem_of_lt {k: Nat} {f: Nat → Fin k} {p q: Nat} (h: p < q
     Vector.mem_toList_iff.mpr Vector.get_mem,
     constructTable_mem_iff.mpr ⟨h, rfl⟩
   ⟩)
-
-
-theorem Vector.exists_get_of_mem {α} {k: Nat} {v: Vector α k} {a: α} (h: a ∈ v):
-    ∃ i: Fin k, a = v.get i :=
-  have ⟨i, hi, hvi⟩ := Vector.mem_iff_getElem.mp h; ⟨⟨i, hi⟩, hvi.symm⟩
 
 
 theorem countingSort'_lt {k: Nat} {f: Nat → Fin k} {n: Nat}:
@@ -332,30 +204,6 @@ theorem countingSort'_mem_iff {k: Nat} {f: Nat → Fin k} {n: Nat}:
 
 
 --Injectivity
-def List.Disjoint {α} (u v: List α): Prop := ∀ a: α, a ∈ u → a ∈ v → False
-
-
-theorem List.nodup_flatten {α} {l: List (List α)}
-  (h1: l.Pairwise List.Disjoint) (h2: ∀ u: List α, u ∈ l → u.Nodup):
-    l.flatten.Nodup :=
-  match l with
-  | [] => List.nodup_nil
-  | h::_ =>
-    List.flatten_cons ▸ List.nodup_append.mpr ⟨
-      h2 h List.mem_cons_self,
-      List.nodup_flatten (List.pairwise_cons.mp h1).right
-        (fun u hu => h2 u (List.mem_cons_of_mem h hu)),
-      fun a ha _ hb eq =>
-        have ⟨u, hu, hb⟩ := List.mem_flatten.mp hb
-        have h_u_disjoint := (List.pairwise_cons.mp h1).left u hu
-        h_u_disjoint a ha (eq ▸ hb)
-    ⟩
-
-
-theorem Vector.getElem_toList' {α} {k: Nat} {v: Vector α k} {i: Fin k}:
-    v.toList[i] = v.get i := Vector.getElem_toList (Vector.length_toList ▸ i.isLt)
-
-
 theorem constructTable_pairwise_disjoint {k: Nat} {f: Nat → Fin k} {n: Nat}:
     (constructTable f n).toList.Pairwise List.Disjoint :=
   List.pairwise_iff_getElem.mpr (fun i j hi hj lt a ha_i ha_j =>
@@ -371,12 +219,6 @@ theorem constructTable_pairwise_disjoint {k: Nat} {f: Nat → Fin k} {n: Nat}:
   )
 
 
-theorem Vector.get_of_mem {α} {k: Nat} {v: Vector α k} {a: α} (h: a ∈ v):
-    ∃ i: Fin k, v.get i = a :=
-  have ⟨i, hi, eq⟩ := Vector.getElem_of_mem h
-  ⟨⟨i, hi⟩, eq⟩
-
-
 theorem countingSort'_nodup {k: Nat} {f: Nat → Fin k} {n: Nat}:
     (countingSort' f n).toList.Nodup :=
   List.toList_toArray ▸ List.nodup_flatten constructTable_pairwise_disjoint (fun _ hu =>
@@ -386,52 +228,6 @@ theorem countingSort'_nodup {k: Nat} {f: Nat → Fin k} {n: Nat}:
 
 
 --Sorting correctness
-theorem List.sublist_flatten_of_sublist {α} {u v: List (List α)}:
-    u.Sublist v → u.flatten.Sublist v.flatten
-  | List.Sublist.slnil => List.Sublist.refl []
-  | List.Sublist.cons (l₂ := t) l h => List.Sublist.trans
-    (List.sublist_flatten_of_sublist h)
-    (List.flatten_cons ▸ (List.sublist_append_right l t.flatten))
-  | List.Sublist.cons₂ l h => (List.append_sublist_append_left l).mpr
-    (List.sublist_flatten_of_sublist h)
-
-
-theorem List.pair_sublist_flatten {α} {a b: α} {l: List (List α)}
-  (h: ∃ u v: List α, a ∈ u ∧ b ∈ v ∧ [u, v].Sublist l):
-    [a, b].Sublist l.flatten :=
-  have ⟨u, v, ha, hb, sub⟩ := h
-  have s₁: [a, b].Sublist (u ++ v) := (List.singleton_sublist.mpr ha).append
-    (List.singleton_sublist.mpr hb)
-  have s₂: [u, v].flatten.Sublist l.flatten := List.sublist_flatten_of_sublist sub
-  have flatten_append: [u, v].flatten = u ++ v := List.flatten_cons.symm ▸ List.flatten_cons.symm ▸
-    List.flatten_nil.symm ▸ (List.append_nil _).symm ▸ rfl
-  s₁.trans (flatten_append ▸ s₂)
-
-
-theorem List.pair_getElem_sublist {α} {l: List α} {i j: Nat}
-  (hi: i < l.length) (hj: j < l.length) (h: i < j):
-    [l[i], l[j]].Sublist l :=
-  have ⟨a, t, hl⟩ := List.exists_cons_of_length_pos (Nat.zero_lt_of_lt hi)
-  have length_l: l.length = t.length + 1 := hl ▸ List.length_cons
-  have ⟨v, hv⟩ := Nat.exists_eq_succ_of_ne_zero (Nat.ne_zero_of_lt h)
-  match i with
-  | 0 =>
-    have htail: [t[v]].Sublist t := List.singleton_sublist.mpr (List.getElem_mem _)
-    have htail': [l[j]].Sublist t := hv ▸ hl ▸ htail
-    have a_eq: a = l[0] := hl ▸ rfl
-    have c: [l[0], l[j]].Sublist (a::t) := a_eq ▸ (List.Sublist.cons₂ a htail'); hl ▸ c
-  | u + 1 =>
-    have u_lt: u < t.length := Nat.lt_of_add_lt_add_right (length_l ▸ hi)
-    have v_lt: v < t.length := Nat.lt_of_add_lt_add_right (length_l ▸ hv ▸ hj)
-    have hrec := List.pair_getElem_sublist u_lt v_lt (Nat.lt_of_add_lt_add_right (hv ▸ h))
-    hl ▸ (List.Sublist.cons a (hv ▸ hrec))
-
-
-theorem Vector.pair_get_sublist_toList {α} {k: Nat} {v: Vector α k} {i j: Fin k} (h: ↑i < ↑j):
-    [v.get i, v.get j].Sublist v.toList :=
-  Vector.getElem_toList' ▸ Vector.getElem_toList' ▸ (List.pair_getElem_sublist _ _ h)
-
-
 theorem countingSort'_order {k: Nat} {f: Nat → Fin k} {p q n: Nat}
   (h: f p < f q) (h1: p < n) (h2: q < n):
     [p, q].Sublist (countingSort' f n).toList :=
@@ -447,12 +243,6 @@ theorem countingSort'_order {k: Nat} {f: Nat → Fin k} {p q n: Nat}
 
 
 --Stability
-theorem List.sublist_flatten_of_sublist_elem {α} {l: List (List α)} {u: List α}
-  (h: ∃ v: List α, v ∈ l ∧ u.Sublist v):
-    u.Sublist l.flatten :=
-  have ⟨_, hv, hu⟩ := h; hu.trans (List.sublist_flatten_of_mem hv)
-
-
 theorem countingSort'_stable {k: Nat} {f: Nat → Fin k} {p q n: Nat}
   (h: f p = f q) (h1: p < q) (h2: q < n):
     [p, q].Sublist (countingSort' f n).toList :=
@@ -492,19 +282,6 @@ theorem countingSort_stable {k: Nat} {f: Nat → Fin k} {p q n: Nat}
 /-
 Radix sort from a given permutation
 -/
-def Array.compose (v w: Array Nat) :=
-  w.map (fun i => v.getD i 0)
-
-
-theorem Array.getElem_compose {v w: Array Nat} {i: Nat} (hi: i < w.size) (hwi: w[i] < v.size):
-    (v.compose w)[i]'(Array.size_map.symm ▸ hi) = v[w[i]] :=
-  (Array.getElem_map _ _) ▸ (Array.getElem_eq_getD 0).symm
-
-
-theorem Array.size_compose {v w: Array Nat}: (v.compose w).size = w.size :=
-  Array.size_map
-
-
 def radixSortFrom {radix: Nat → Nat} (f: Nat → (r: Nat) → Fin (radix r)) (v: Array Nat):
     (s: Nat) → Array Nat
   | 0 => v
@@ -514,7 +291,7 @@ def radixSortFrom {radix: Nat → Nat} (f: Nat → (r: Nat) → Fin (radix r)) (
 --Surjectivity
 theorem countingSort_size {k: Nat} {f: Nat → Fin k} {n: Nat}:
     (countingSort f n).size = n :=
-  Array.length_toList ▸ perm_length_eq (fun i => ⟨
+  Array.length_toList ▸ List.perm_length_eq (fun i => ⟨
     fun hi => Array.mem_toList_iff.mpr ((countingSort_mem_iff i).mpr hi),
     fun hi => ((countingSort_mem_iff i).mp (Array.mem_toList_iff.mp hi)),
   ⟩) countingSort_nodup
@@ -542,24 +319,6 @@ theorem radixSortFrom_mem_iff {radix: Nat → Nat} {f: Nat → (r: Nat) → Fin 
     ) p
 
 --Injectivity
-theorem Array.compose_nodup {v w: Array Nat} (h1: v.toList.Nodup) (h2: w.toList.Nodup)
-  (h3: ∀ i: Nat, i ∈ w → i < v.size):
-    (v.compose w).toList.Nodup :=
-  List.pairwise_iff_getElem.mpr (fun i j hi hj hij eq =>
-    have hi: i < w.size := Array.size_map ▸ Array.length_toList ▸ hi
-    have hj: j < w.size := Array.size_map ▸ Array.length_toList ▸ hj
-    have hwi: w[i] < v.size := h3 w[i] (Array.getElem_mem hi)
-    have hwj: w[j] < v.size := h3 w[j] (Array.getElem_mem hj)
-    have eqi: (v.compose w).toList[i] = v[w[i]] := Array.getElem_compose hi hwi
-    have eqj: (v.compose w).toList[j] = v[w[j]] := Array.getElem_compose hj hwj
-    have eq: v[w[i]] = v[w[j]] := eqi ▸ eqj ▸ eq
-    match Nat.lt_trichotomy w[i] w[j] with
-    | .inl ineq => List.pairwise_iff_getElem.mp h1 w[i] w[j] hwi hwj ineq eq
-    | .inr (.inl eq) => List.pairwise_iff_getElem.mp h2 i j hi hj hij eq
-    | .inr (.inr ineq) => List.pairwise_iff_getElem.mp h1 w[j] w[i] hwj hwi ineq eq.symm
-  )
-
-
 theorem radixSortFrom_nodup {radix: Nat → Nat} {f: Nat → (r: Nat) → Fin (radix r)}
   {v: Array Nat} (h: v.toList.Nodup):
     {s: Nat} → (radixSortFrom f v s).toList.Nodup
@@ -569,48 +328,16 @@ theorem radixSortFrom_nodup {radix: Nat → Nat} {f: Nat → (r: Nat) → Fin (r
 
 
 --Sorting correctness
-def lexEq {radix: Nat → Nat} (f g: (r: Nat) → Fin (radix r)) (r: Nat): Prop :=
+@[expose]
+public def lexEq {radix: Nat → Nat} (f g: (r: Nat) → Fin (radix r)) (r: Nat): Prop :=
   ∀ i: Nat, i < r → f i = g i
 
 
-def lexLt {radix: Nat → Nat} (f g: (r: Nat) → Fin (radix r)):
+@[expose]
+public def lexLt {radix: Nat → Nat} (f g: (r: Nat) → Fin (radix r)):
     Nat → Prop
   | 0 => False
   | r + 1 => (lexLt f g r) ∨ ((lexEq f g r) ∧ (f r < g r))
-
-
-theorem List.exists_pair_getElem_of_sublist {α} {l: List α} {a b: α} (h: [a, b].Sublist l):
-    ∃ ia ib: Nat, ∃ hia: ia < ib, ∃ hib: ib < l.length, l[ia] = a ∧ l[ib] = b :=
-  have ⟨ra, rb, hr, amem, sub⟩ := List.cons_sublist_iff.mp h
-  have bmem := List.singleton_sublist.mp sub
-  have ⟨ria, hria, eqa⟩ := List.getElem_of_mem amem
-  have ⟨rib, hrib, eqb⟩ := List.getElem_of_mem bmem
-  ⟨
-    ria, rib + ra.length,
-    Nat.lt_add_left _ hria,
-    hr.symm ▸ List.length_append ▸ Nat.add_comm _ _ ▸ Nat.add_lt_add_left hrib _,
-    hr.symm ▸ eqa ▸ List.getElem_append_left hria,
-    hr.symm ▸ eqb ▸ (List.getElem_append_right' ra hrib).symm
-  ⟩
-
-
-theorem Array.compose_sublist_pair {v w: Array Nat} {a b: Nat} (h1: [a, b].Sublist w.toList)
-  (h2: a < v.size) (h3: b < v.size):
-    [v[a], v[b]].Sublist (v.compose w).toList :=
-  have ⟨ia, ib, hia, hib, eqa, eqb⟩ := List.exists_pair_getElem_of_sublist h1
-  have hib: ib < w.size := Array.length_toList ▸ hib
-  have eqa: w[ia] = a := eqa; have eqb: w[ib] = b := eqb
-  have size_eq: (v.compose w).toList.length = w.toList.length :=
-    Array.length_toList ▸ Array.length_toList ▸ Array.size_compose
-  have hia': ia < (v.compose w).toList.length := size_eq ▸ Nat.lt_trans hia hib
-  have hib': ib < (v.compose w).toList.length := size_eq ▸ hib
-  have veqa: v[w[ia]] = v[a] := getElem_congr_idx eqa
-  have veqb: v[w[ib]] = v[b] := getElem_congr_idx eqb
-  have eqa': (v.compose w).toList[ia] = v[a] :=
-    veqa ▸ Array.getElem_toList _ ▸ (Array.getElem_compose (Nat.lt_trans hia hib) (eqa ▸ h2))
-  have eqb': (v.compose w).toList[ib] = v[b] :=
-    veqb ▸ Array.getElem_toList _ ▸ (Array.getElem_compose hib (eqb ▸ h3))
-  eqa' ▸ eqb' ▸ List.pair_getElem_sublist hia' hib' hia
 
 
 theorem radixSortFrom_stable {radix: Nat → Nat} {f: Nat → (r: Nat) → Fin (radix r)} {v: Array Nat}
@@ -628,12 +355,6 @@ theorem radixSortFrom_stable {radix: Nat → Nat} {f: Nat → (r: Nat) → Fin (
     radixSortFrom_stable (s := s) (fun i hi => h1 i (Nat.lt_succ_of_lt hi))
       (eqp ▸ eqq ▸ Array.compose_sublist_pair
         (countingSort_stable f_eq hip hiq) (Nat.lt_trans hip hiq) hiq)
-
-
-theorem Array.mem_compose_of_mem {v w: Array Nat} {n: Nat} (h1: n ∈ v)
-  (h2: ∀ i: Nat, i < v.size → i ∈ w): n ∈ v.compose w :=
-  have ⟨i, hi, eq⟩ := Array.getElem_of_mem h1
-  Array.mem_map.mpr ⟨i, h2 i hi, Array.getElem_eq_getD 0 ▸ eq⟩
 
 
 theorem radixSortFrom_order {radix: Nat → Nat} {f: Nat → (r: Nat) → Fin (radix r)} {v: Array Nat}
@@ -658,11 +379,11 @@ theorem radixSortFrom_order {radix: Nat → Nat} {f: Nat → (r: Nat) → Fin (r
 Radix sort
 -/
 
-def radixSort {radix: Nat → Nat} (f: Nat → (r: Nat) → Fin (radix r)) (n: Nat): Nat → Array Nat :=
+public def radixSort {radix: Nat → Nat} (f: Nat → (r: Nat) → Fin (radix r)) (n: Nat): Nat → Array Nat :=
   radixSortFrom f (Array.range n)
 
 
-theorem radixSort_mem_iff {radix: Nat → Nat} {f: Nat → (r: Nat) → Fin (radix r)} {n s: Nat}:
+public theorem radixSort_mem_iff {radix: Nat → Nat} {f: Nat → (r: Nat) → Fin (radix r)} {n s: Nat}:
     ∀ p: Nat, p < n ↔ p ∈ radixSort f n s :=
   have concl: ∀ p: Nat, p < (Array.range n).size ↔ p ∈ radixSort f n s :=
     radixSortFrom_mem_iff  (fun _ => Array.size_range ▸ Array.mem_range.symm)
@@ -672,22 +393,23 @@ theorem radixSort_mem_iff {radix: Nat → Nat} {f: Nat → (r: Nat) → Fin (rad
   ⟩
 
 
-theorem radixSort_nodup {radix: Nat → Nat} {f: Nat → (r: Nat) → Fin (radix r)} {n s: Nat}:
+public theorem radixSort_nodup {radix: Nat → Nat} {f: Nat → (r: Nat) → Fin (radix r)} {n s: Nat}:
     (radixSort f n s).toList.Nodup :=
   radixSortFrom_nodup (Array.toList_range ▸ List.nodup_range)
 
 
-theorem radixSort_order {radix: Nat → Nat} {f: Nat → (r: Nat) → Fin (radix r)} {n: Nat}
+public theorem radixSort_order {radix: Nat → Nat} {f: Nat → (r: Nat) → Fin (radix r)} {n: Nat}
   {p q s: Nat} (h: lexLt (f p) (f q) s) (h1: p < n) (h2: q < n):
     [p, q].Sublist (radixSort f n s).toList :=
   radixSortFrom_order h (Array.mem_range.mpr h1) (Array.mem_range.mpr h2)
 
 --More traditional formulation of correctness, easier to use
-def lexLe {radix: Nat → Nat} (f g: (r: Nat) → Fin (radix r)) (n: Nat): Prop :=
+@[expose]
+public def lexLe {radix: Nat → Nat} (f g: (r: Nat) → Fin (radix r)) (n: Nat): Prop :=
   lexLt f g n ∨ lexEq f g n
 
 
-theorem lexLe_or_lexLt {radix: Nat → Nat} (f g: (r: Nat) → Fin (radix r)):
+public theorem lexLe_or_lexLt {radix: Nat → Nat} (f g: (r: Nat) → Fin (radix r)):
      (n: Nat) → lexLe f g n ∨ lexLt g f n
   | 0 => Or.inl (Or.inr (fun i hi => False.elim (Nat.not_lt_zero i hi)))
   | n + 1 => match lexLe_or_lexLt f g n with
@@ -703,23 +425,15 @@ theorem lexLe_or_lexLt {radix: Nat → Nat} (f g: (r: Nat) → Fin (radix r)):
     | .inr lt => Or.inr (Or.inl lt)
 
 
-theorem radixSort_size {radix: Nat → Nat} {f: Nat → (r: Nat) → Fin (radix r)} {n s: Nat}:
+public theorem radixSort_size {radix: Nat → Nat} {f: Nat → (r: Nat) → Fin (radix r)} {n s: Nat}:
    (radixSort f n s).size = n :=
-  perm_length_eq (fun p => ⟨
+  List.perm_length_eq (fun p => ⟨
     fun hp => Array.mem_toList_iff.mpr ((radixSort_mem_iff p).mp hp),
     fun hp => (radixSort_mem_iff p).mpr (Array.mem_toList_iff.mp hp)
   ⟩) radixSort_nodup
 
 
-theorem List.idx_inj_of_nodup {α} {l: List α} (h1: l.Nodup) {i j: Nat} (hi: i < l.length) (hj: j < l.length)
-    (h2: l[i] = l[j]): i = j :=
-  match Nat.lt_trichotomy i j with
-  | .inl lt => False.elim (List.pairwise_iff_getElem.mp h1 i j hi hj lt h2)
-  | .inr (.inl eq) => eq
-  | .inr (.inr lt) => False.elim (List.pairwise_iff_getElem.mp h1 j i hj hi lt h2.symm)
-
-
-theorem radixSort_order' {radix: Nat → Nat} {f: Nat → (r: Nat) → Fin (radix r)} {n: Nat}
+public theorem radixSort_order' {radix: Nat → Nat} {f: Nat → (r: Nat) → Fin (radix r)} {n: Nat}
   {i j s: Nat} (hi: i < n) (hj: j < n) (h: i ≤ j):
     lexLe
       (f ((radixSort f n s)[i]'(radixSort_size ▸ hi)))
