AutoKchp.lean
@@ -1,0 +1,4 @@
+module
+
+public import AutoKchp.NatCDFA
+public import AutoKchp.MorphismDfs
