AutoKchp/NatCDFA.lean
@@ -1,0 +1,82 @@
+module
+
+import AutoKchp.Util
+
+@[expose]
+public section
+
+structure NatCDFA (a: Nat) where
+  n: Nat
+  δ: Fin n → Fin a → Fin n
+  i: Fin n
+  f: Fin n → Bool
+
+namespace NatCDFA
+
+def advanceFrom {a: Nat} (r: NatCDFA a) (q: Fin r.n): List (Fin a) → Fin r.n
+  | a::t => r.advanceFrom (r.δ q a) t
+  | [] => q
+
+
+def acceptsFrom {a: Nat} (r: NatCDFA a) (q: Fin r.n) (w: List (Fin a)): Bool :=
+  r.f (r.advanceFrom q w)
+
+
+def advance {a: Nat} (r: NatCDFA a): List (Fin a) → Fin r.n := r.advanceFrom r.i
+
+
+def accepts {a: Nat} (r: NatCDFA a): List (Fin a) → Bool := r.acceptsFrom r.i
+
+
+def concretize {a: Nat} (r: NatCDFA a): NatCDFA a :=
+  let transitions := Vector.ofFn (fun i => Vector.ofFn (fun b => r.δ i b))
+  let final := Vector.ofFn r.f
+  {
+    n := r.n
+    δ := fun i b => (transitions.get i).get b
+    i := r.i
+    f := fun i => final.get i
+  }
+
+
+theorem concretize_id {a: Nat} {r: NatCDFA a}: r.concretize = r :=
+  r.casesOn (fun n δ i t => mk.injEq _ _ _ _ n δ i t ▸ ⟨
+      rfl,
+      heq_of_eq (funext fun _ => (funext fun _ => Vector.get_ofFn ▸ Vector.get_ofFn)),
+      heq_of_eq rfl,
+      heq_of_eq (funext fun _ => Vector.get_ofFn)
+    ⟩
+  )
+
+
+theorem advanceFrom_append {a: Nat} {r: NatCDFA a} {q: Fin r.n} {f₁ f₂: List (Fin a)}:
+    r.advanceFrom q (f₁ ++ f₂) = r.advanceFrom (r.advanceFrom q f₁) f₂ :=
+  match f₁ with
+  | [] => rfl
+  | _::_ => List.cons_append ▸ NatCDFA.advanceFrom_append
+
+
+theorem advanceFrom_concat {a: Nat} {r: NatCDFA a} {q: Fin r.n} {f: List (Fin a)} {b: Fin a}:
+    r.advanceFrom q (f ++ [b]) = r.δ (r.advanceFrom q f) b :=
+  NatCDFA.advanceFrom_append
+
+
+theorem advance_concat {a: Nat} {r: NatCDFA a} {f: List (Fin a)} {b: Fin a}:
+    r.advance (f ++ [b]) = r.δ (r.advance f) b :=
+  NatCDFA.advanceFrom_concat
+
+
+def morphism {a: Nat} (r s: NatCDFA a) (f: Fin r.n → Fin s.n): Prop :=
+  ∀ l: List (Fin a), f (r.advance l) = s.advance l ∧ r.accepts l = s.accepts l
+
+
+def existsMorphism {a: Nat} (r s: NatCDFA a): Prop :=
+  ∃ f: Fin r.n → Fin s.n, NatCDFA.morphism r s f
+
+
+def minimal {a: Nat} (r: NatCDFA a): Prop :=
+  ∀ s: NatCDFA a, s.accepts = r.accepts → NatCDFA.existsMorphism s r
+
+
+end NatCDFA
+end
