AutoKchp/Util.lean
@@ -1,0 +1,449 @@
+module
+
+@[expose]
+public section
+namespace List
+
+variable {α}
+
+def Disjoint (u v: List α): Prop := ∀ a: α, a ∈ u → a ∈ v → False
+
+
+theorem nodup_singleton {a: α}: [a].Nodup :=
+  nodup_cons.mpr ⟨not_mem_nil, nodup_nil⟩
+
+
+theorem nodup_append_singleton {l: List α} {a: α} (h1: a ∉ l) (h2: l.Nodup):
+    (l ++ [a]).Nodup :=
+  nodup_append.mpr ⟨h2, nodup_singleton,
+    fun _ hx _ hy hxy => h1 ((hxy ▸ (mem_singleton.mp hy)) ▸ hx)⟩
+
+
+theorem flatten_append_eq_foldl_append {u: List α}:
+    {l: List (List α)} → u ++ l.flatten = l.foldl (fun acc v => acc ++ v) u
+  | [] => flatten_nil ▸ append_nil _ ▸ foldl_nil ▸ rfl
+  | _::_ => flatten_cons.symm ▸ (append_assoc _ _ _ ▸ flatten_append_eq_foldl_append)
+
+
+theorem flatten_eq_foldl_append {l: List (List α)}:
+    l.flatten = l.foldl (fun acc u => acc ++ u) [] :=
+  flatten_append_eq_foldl_append ▸ nil_append _
+
+
+theorem concat_eq_foldl {u: List α}:
+    {v: List α} → u ++ v = v.foldl (fun acc a => acc ++ [a]) u
+  | [] => (append_nil _).symm ▸ (foldl_nil ▸ rfl)
+  | _::_ => foldl_cons.symm ▸ concat_eq_foldl ▸ (append_cons u _ _) ▸ rfl
+
+
+theorem flatten_eq_foldl_foldl {l: List (List α)}:
+    l.flatten = l.foldl (fun acc u => u.foldl (fun acc a => acc ++ [a]) acc) [] :=
+  flatten_eq_foldl_append ▸ congrArg
+    (fun x => l.foldl x [])
+    (funext (fun _ => funext (fun _ => concat_eq_foldl)))
+
+
+theorem nodup_flatten {l: List (List α)}
+  (h1: l.Pairwise Disjoint) (h2: ∀ u: List α, u ∈ l → u.Nodup):
+    l.flatten.Nodup :=
+  match l with
+  | [] => nodup_nil
+  | h::_ =>
+    flatten_cons ▸ nodup_append.mpr ⟨
+      h2 h mem_cons_self,
+      nodup_flatten (pairwise_cons.mp h1).right
+        (fun u hu => h2 u (mem_cons_of_mem h hu)),
+      fun a ha _ hb eq =>
+        have ⟨u, hu, hb⟩ := mem_flatten.mp hb
+        have h_u_disjoint := (pairwise_cons.mp h1).left u hu
+        h_u_disjoint a ha (eq ▸ hb)
+    ⟩
+
+
+theorem sublist_flatten_of_sublist {u v: List (List α)}:
+    u.Sublist v → u.flatten.Sublist v.flatten
+  | Sublist.slnil => Sublist.refl []
+  | Sublist.cons (l₂ := t) l h => Sublist.trans
+    (sublist_flatten_of_sublist h)
+    (flatten_cons ▸ (sublist_append_right l t.flatten))
+  | Sublist.cons₂ l h => (append_sublist_append_left l).mpr
+    (sublist_flatten_of_sublist h)
+
+
+theorem pair_sublist_flatten {a b: α} {l: List (List α)}
+  (h: ∃ u v: List α, a ∈ u ∧ b ∈ v ∧ [u, v].Sublist l):
+    [a, b].Sublist l.flatten :=
+  have ⟨u, v, ha, hb, sub⟩ := h
+  have s₁: [a, b].Sublist (u ++ v) := (singleton_sublist.mpr ha).append
+    (singleton_sublist.mpr hb)
+  have s₂: [u, v].flatten.Sublist l.flatten := sublist_flatten_of_sublist sub
+  have flatten_append: [u, v].flatten = u ++ v := flatten_cons.symm ▸ flatten_cons.symm ▸
+    flatten_nil.symm ▸ (append_nil _).symm ▸ rfl
+  s₁.trans (flatten_append ▸ s₂)
+
+
+theorem pair_getElem_sublist {l: List α} {i j: Nat}
+  (hi: i < l.length) (hj: j < l.length) (h: i < j):
+    [l[i], l[j]].Sublist l :=
+  have ⟨a, t, hl⟩ := exists_cons_of_length_pos (Nat.zero_lt_of_lt hi)
+  have length_l: l.length = t.length + 1 := hl ▸ length_cons
+  have ⟨v, hv⟩ := Nat.exists_eq_succ_of_ne_zero (Nat.ne_zero_of_lt h)
+  match i with
+  | 0 =>
+    have htail: [t[v]].Sublist t := singleton_sublist.mpr (getElem_mem _)
+    have htail': [l[j]].Sublist t := hv ▸ hl ▸ htail
+    have a_eq: a = l[0] := hl ▸ rfl
+    have c: [l[0], l[j]].Sublist (a::t) := a_eq ▸ (Sublist.cons₂ a htail'); hl ▸ c
+  | u + 1 =>
+    have u_lt: u < t.length := Nat.lt_of_add_lt_add_right (length_l ▸ hi)
+    have v_lt: v < t.length := Nat.lt_of_add_lt_add_right (length_l ▸ hv ▸ hj)
+    have hrec := pair_getElem_sublist u_lt v_lt (Nat.lt_of_add_lt_add_right (hv ▸ h))
+    hl ▸ (Sublist.cons a (hv ▸ hrec))
+
+
+theorem sublist_flatten_of_sublist_elem {l: List (List α)} {u: List α}
+  (h: ∃ v: List α, v ∈ l ∧ u.Sublist v):
+    u.Sublist l.flatten :=
+  have ⟨_, hv, hu⟩ := h; hu.trans (List.sublist_flatten_of_mem hv)
+
+
+theorem exists_pair_getElem_of_sublist {l: List α} {a b: α} (h: [a, b].Sublist l):
+    ∃ ia ib: Nat, ∃ hia: ia < ib, ∃ hib: ib < l.length, l[ia] = a ∧ l[ib] = b :=
+  have ⟨ra, rb, hr, amem, sub⟩ := List.cons_sublist_iff.mp h
+  have bmem := List.singleton_sublist.mp sub
+  have ⟨ria, hria, eqa⟩ := List.getElem_of_mem amem
+  have ⟨rib, hrib, eqb⟩ := List.getElem_of_mem bmem
+  ⟨
+    ria, rib + ra.length,
+    Nat.lt_add_left _ hria,
+    hr.symm ▸ List.length_append ▸ Nat.add_comm _ _ ▸ Nat.add_lt_add_left hrib _,
+    hr.symm ▸ eqa ▸ List.getElem_append_left hria,
+    hr.symm ▸ eqb ▸ (List.getElem_append_right' ra hrib).symm
+  ⟩
+
+
+theorem idx_inj_of_nodup {l: List α} (h1: l.Nodup) {i j: Nat} (hi: i < l.length) (hj: j < l.length)
+    (h2: l[i] = l[j]): i = j :=
+  match Nat.lt_trichotomy i j with
+  | .inl lt => False.elim (List.pairwise_iff_getElem.mp h1 i j hi hj lt h2)
+  | .inr (.inl eq) => eq
+  | .inr (.inr lt) => False.elim (List.pairwise_iff_getElem.mp h1 j i hj hi lt h2.symm)
+
+end List
+end
+
+
+public section
+namespace Vector
+
+variable {α} {k: Nat}
+
+def modify (v: Vector α k) (i: Fin k) (f: α → α): Vector α k :=
+  ⟨v.toArray.modify i.val f, Eq.trans Array.size_modify v.size_toArray⟩
+
+
+theorem get_modify_self {v: Vector α k} {i: Fin k} {f: α → α}:
+    (v.modify i f).get i = f (v.get i) :=
+  Array.getElem_modify_self f ((v.modify i f).size_toArray.symm ▸ i.isLt)
+
+
+theorem get_modify_of_ne {v: Vector α k} {i j: Fin k} {f: α → α} (h: i ≠ j):
+    (v.modify i f).get j = v.get j :=
+  Array.getElem_modify_of_ne (Fin.val_ne_iff.mpr h) f ((v.modify i f).size_toArray.symm ▸ j.isLt)
+
+
+theorem get_ext {v w: Vector α k} (h: ∀ i: Fin k, v.get i = w.get i): v = w :=
+  Vector.ext (fun i hi => h ⟨i, hi⟩)
+
+
+theorem get_replicate {a: α} {i: Fin k}: (replicate k a).get i = a :=
+  have lt: i.val < (replicate k a).toArray.size :=
+    ((replicate k a).size_toArray.symm) ▸ i.isLt
+  Array.getElem_replicate lt
+
+
+theorem modify_modify_self {v: Vector α k} {i: Fin k} {f g: α → α}:
+    (v.modify i f).modify i g = v.modify i (g ∘ f) :=
+  get_ext (fun j =>
+    if eq: i = j then
+        eq.symm ▸
+        get_modify_self.symm ▸
+        get_modify_self.symm ▸
+        get_modify_self.symm ▸ rfl
+    else
+        (get_modify_of_ne eq).symm ▸
+        (get_modify_of_ne eq).symm ▸
+        (get_modify_of_ne eq).symm ▸ rfl
+  )
+
+
+theorem modify_modify_of_ne {v: Vector α k} {i j: Fin k} {f g: α → α} (h: i ≠ j):
+    (v.modify i f).modify j g = (v.modify j g).modify i f :=
+  get_ext (fun a =>
+    if eqi: i = a then
+      eqi ▸
+      (get_modify_of_ne h.symm).symm ▸
+      get_modify_self.symm ▸
+      get_modify_self.symm ▸
+      (get_modify_of_ne h.symm).symm ▸ rfl
+    else if eqj: j = a then
+      eqj ▸
+      (get_modify_of_ne h).symm ▸
+      get_modify_self.symm ▸
+      get_modify_self.symm ▸
+      (get_modify_of_ne h).symm ▸ rfl
+    else
+      (get_modify_of_ne eqi).symm ▸
+      (get_modify_of_ne eqj).symm ▸
+      (get_modify_of_ne eqj).symm ▸
+      (get_modify_of_ne eqi).symm ▸ rfl
+  )
+
+
+theorem modify_comm {v: Vector α k} {i j: Fin k}
+  {f: α → α} {g: α → α} (h: g ∘ f = f ∘ g):
+    (v.modify i f).modify j g = (v.modify j g).modify i f :=
+  if eq: i = j then
+    eq ▸
+    modify_modify_self.symm ▸
+    modify_modify_self.symm ▸
+    (congrArg _ h)
+  else
+    modify_modify_of_ne eq
+
+
+theorem get_ofFn {f: Fin k → α} {i: Fin k}:
+    (ofFn f).get i = f i :=
+  Array.getElem_ofFn _
+
+
+theorem get_mem {v: Vector α k} {i: Fin k}: v.get i ∈ v :=
+    Vector.getElem_mem i.isLt
+
+
+theorem exists_get_of_mem {v: Vector α k} {a: α} (h: a ∈ v):
+    ∃ i: Fin k, a = v.get i :=
+  have ⟨i, hi, hvi⟩ := Vector.mem_iff_getElem.mp h; ⟨⟨i, hi⟩, hvi.symm⟩
+
+
+theorem getElem_toList' {v: Vector α k} {i: Fin k}:
+    v.toList[i] = v.get i := Vector.getElem_toList (Vector.length_toList ▸ i.isLt)
+
+
+theorem get_of_mem {v: Vector α k} {a: α} (h: a ∈ v):
+    ∃ i: Fin k, v.get i = a :=
+  have ⟨i, hi, eq⟩ := Vector.getElem_of_mem h
+  ⟨⟨i, hi⟩, eq⟩
+
+
+theorem pair_get_sublist_toList {v: Vector α k} {i j: Fin k} (h: ↑i < ↑j):
+    [v.get i, v.get j].Sublist v.toList :=
+  Vector.getElem_toList' ▸ Vector.getElem_toList' ▸ (List.pair_getElem_sublist _ _ h)
+
+
+def cNone (v: Vector (Option α) k) := v.countP Option.isNone
+
+
+theorem cNone_set {v: Vector (Option α) k} {i: Fin k} {x: α}
+  (h: v.get i = none):
+    (v.set i x).cNone + 1 = v.cNone :=
+  have cond: v[i.val].isNone = true := Option.isNone_iff_eq_none.mpr h
+  have le: v.countP Option.isNone ≥ 1 := Nat.one_le_of_lt (countP_pos_iff.mpr
+    ⟨v.get i, getElem_mem _, Option.isNone_iff_eq_none.mpr h⟩)
+  (congrArg (· + 1) (countP_set i.isLt)).trans (
+    ite_cond_eq_true _ _ (eq_true cond) ▸ Nat.sub_add_comm le ▸
+    (Nat.sub_add_cancel (Nat.le_add_right_of_le le)).symm ▸ rfl)
+
+
+theorem cNone_le {v: Vector (Option α) k}: v.cNone ≤ k :=
+  Vector.countP_le_size
+
+
+theorem get_set_self {v: Vector α k} {i: Fin k} {a: α}:
+    (v.set i a).get i = a :=
+  getElem_set_self i.isLt
+
+
+theorem get_set_of_ne {v: Vector α k} {i j: Fin k} {a: α} (h: i ≠ j):
+    (v.set i a).get j = v.get j :=
+  getElem_set_ne i.isLt j.isLt (Fin.val_ne_of_ne h)
+
+end Vector
+end
+
+
+@[expose]
+public section
+namespace Array
+
+def flattenLists {α} {v: Array (List α)}: Array α :=
+  v.foldl (fun acc l => l.foldl (fun acc a => acc.push a) acc) empty
+
+
+theorem toList_flattenLists {α} {v: Array (List α)}:
+    v.flattenLists.toList = v.foldl (fun acc l => l.foldl (fun acc a => acc ++ [a]) acc) [] :=
+  (foldl_hom toList fun _ _ => (
+    List.foldl_hom toList fun _ _ => Eq.symm toList_push
+  )).symm
+
+
+theorem toList_flattenLists_eq_flatten_toList {α} {v: Array (List α)}:
+    v.flattenLists.toList = v.toList.flatten :=
+  Eq.trans ((foldl_toList _) ▸ toList_flattenLists) List.flatten_eq_foldl_foldl.symm
+
+
+def compose (v w: Array Nat) :=
+  w.map (fun i => v.getD i 0)
+
+
+theorem size_compose {v w: Array Nat}: (v.compose w).size = w.size :=
+  Array.size_map
+
+
+theorem getElem_compose {v w: Array Nat} {i: Nat} (hi: i < w.size) (hwi: w[i] < v.size):
+    (v.compose w)[i]'(size_compose.symm ▸ hi) = v[w[i]] :=
+  (getElem_map _ _) ▸ (getElem_eq_getD 0).symm
+
+
+theorem mem_compose_of_mem {v w: Array Nat} {n: Nat} (h1: n ∈ v)
+  (h2: ∀ i: Nat, i < v.size → i ∈ w): n ∈ v.compose w :=
+  have ⟨i, hi, eq⟩ := getElem_of_mem h1
+  mem_map.mpr ⟨i, h2 i hi, getElem_eq_getD 0 ▸ eq⟩
+
+
+theorem compose_nodup {v w: Array Nat} (h1: v.toList.Nodup) (h2: w.toList.Nodup)
+  (h3: ∀ i: Nat, i ∈ w → i < v.size):
+    (v.compose w).toList.Nodup :=
+  List.pairwise_iff_getElem.mpr (fun i j hi hj hij eq =>
+    have hi: i < w.size := size_map ▸ length_toList ▸ hi
+    have hj: j < w.size := size_map ▸ length_toList ▸ hj
+    have hwi: w[i] < v.size := h3 w[i] (getElem_mem hi)
+    have hwj: w[j] < v.size := h3 w[j] (getElem_mem hj)
+    have eqi: (v.compose w).toList[i] = v[w[i]] := getElem_compose hi hwi
+    have eqj: (v.compose w).toList[j] = v[w[j]] := getElem_compose hj hwj
+    have eq: v[w[i]] = v[w[j]] := eqi ▸ eqj ▸ eq
+    match Nat.lt_trichotomy w[i] w[j] with
+    | .inl ineq => List.pairwise_iff_getElem.mp h1 w[i] w[j] hwi hwj ineq eq
+    | .inr (.inl eq) => List.pairwise_iff_getElem.mp h2 i j hi hj hij eq
+    | .inr (.inr ineq) => List.pairwise_iff_getElem.mp h1 w[j] w[i] hwj hwi ineq eq.symm
+  )
+
+
+theorem compose_sublist_pair {v w: Array Nat} {a b: Nat} (h1: [a, b].Sublist w.toList)
+  (h2: a < v.size) (h3: b < v.size):
+    [v[a], v[b]].Sublist (v.compose w).toList :=
+  have ⟨ia, ib, hia, hib, eqa, eqb⟩ := List.exists_pair_getElem_of_sublist h1
+  have hib: ib < w.size := length_toList ▸ hib
+  have eqa: w[ia] = a := eqa; have eqb: w[ib] = b := eqb
+  have size_eq: (v.compose w).toList.length = w.toList.length :=
+    length_toList ▸ length_toList ▸ size_compose
+  have hia': ia < (v.compose w).toList.length := size_eq ▸ Nat.lt_trans hia hib
+  have hib': ib < (v.compose w).toList.length := size_eq ▸ hib
+  have veqa: v[w[ia]] = v[a] := getElem_congr_idx eqa
+  have veqb: v[w[ib]] = v[b] := getElem_congr_idx eqb
+  have eqa': (v.compose w).toList[ia] = v[a] :=
+    veqa ▸ getElem_toList _ ▸ (getElem_compose (Nat.lt_trans hia hib) (eqa ▸ h2))
+  have eqb': (v.compose w).toList[ib] = v[b] :=
+    veqb ▸ getElem_toList _ ▸ (getElem_compose hib (eqb ▸ h3))
+  eqa' ▸ eqb' ▸ List.pair_getElem_sublist hia' hib' hia
+
+
+theorem getD_eq_default {α} (v: Array α) (d: α) {n: Nat} (h: v.size ≤ n): v.getD n d = d :=
+  dite_cond_eq_false (eq_false (Nat.not_lt_of_le h))
+
+
+theorem back?_eq_back {α} {v: Array α} (h: 0 < v.size): v.back? = some v.back :=
+  (back?_eq_getElem?.trans (getElem?_eq_getElem (Nat.sub_one_lt_of_lt h))).trans
+    (congrArg some (back_eq_getElem _).symm)
+
+end Array
+end
+
+
+@[expose]
+public section
+namespace Option
+
+variable {α}
+
+def allP (p: α → Prop): (o: Option α) → Prop
+  | none => True
+  | some a => p a
+
+
+theorem allP_mp {p q: α → Prop} {o: Option α} (h1: o.allP p) (h2: ∀ a: α, p a → q a): o.allP q :=
+  match o with
+  | none => True.intro
+  | some a => h2 a h1
+
+end Option
+end
+
+
+@[expose]
+public section
+namespace Except
+
+variable {α β}
+
+def allP (p: α → Prop): (e: Except β α) → Prop
+  | Except.error _ => True
+  | Except.ok a => p a
+
+
+def allEP (p: β → Prop): (e: Except β α) → Prop
+  | Except.error e => p e
+  | Except.ok _ => True
+
+
+theorem allP_mp {p q: α → Prop} {e: Except β α} (h1: e.allP p) (h2: ∀ a: α, p a → q a): e.allP q :=
+  match e with
+  | Except.error _ => True.intro
+  | Except.ok a => h2 a h1
+
+
+theorem allP_forall {ι} {p: ι → α → Prop}:
+    {e: Except β α} → (∀ i, e.allP (p i)) ↔ (e.allP (fun a => ∀ i, p i a))
+  | Except.error _ => ⟨fun _ => True.intro, fun _ _ => True.intro⟩
+  | Except.ok _ => ⟨id, id⟩
+
+
+theorem allP_imp {c: Prop} {p: α → Prop}:
+    {e: Except β α} → (c → e.allP p) ↔ (e.allP (fun a => c → p a))
+  | Except.error _ => ⟨fun _ => True.intro, fun _ _ => True.intro⟩
+  | Except.ok _ => ⟨id, id⟩
+
+
+theorem allP_and {p q: α → Prop}: {e: Except β α} → e.allP p ∧ e.allP q ↔ e.allP (fun a => p a ∧ q a)
+  | Except.error _ => ⟨fun _ => True.intro, fun _ => ⟨True.intro, True.intro⟩⟩
+  | Except.ok _ => ⟨id, id⟩
+
+
+theorem pure_def {a: α}: (pure a: Except β α) = Except.ok a := rfl
+
+end Except
+end
+
+
+public theorem Fin.foldl_induction {α} {n: Nat} (motive: α → Nat → Prop)
+  {init: α} (h0: motive init 0) {f: α → Fin n → α}
+  (hr: ∀ (a: α) (i: Fin n), motive a i.val → motive (f a i) i.val.succ):
+    motive (Fin.foldl n f init) n :=
+  match n with
+  | 0 => Fin.foldl_zero _ _ ▸ h0
+  | n + 1 =>
+    have hrec: motive (Fin.foldl n (fun a i => f a i.castSucc) init) n :=
+      Fin.foldl_induction _ h0 (fun a i ha => hr a i.castSucc ha)
+    Fin.foldl_succ_last _ _ ▸ hr _ (last n) hrec
+
+
+public theorem Fin.foldlM_induction {α m} [Monad m] [LawfulMonad m] {n: Nat} (motive: m α → Nat → Prop)
+  {init: α} (h0: motive (pure init) 0) {f: α → Fin n → m α}
+  (hr: ∀ (a: m α) (i: Fin n), motive a i.val → motive (a >>= (f · i)) i.val.succ):
+    motive (Fin.foldlM n f init) n :=
+  match n with
+  | 0 =>  (congrFun (Fin.foldlM_zero f) init).symm.subst (motive := fun w => motive w 0) h0
+  | n + 1 =>
+    have hrec: motive (Fin.foldlM n (fun a i => f a i.castSucc) init) n :=
+      Fin.foldlM_induction _ h0 (fun a i ha => hr a i.castSucc ha)
+    Fin.foldlM_succ_last (m := m) _ ▸ hr _ (last n) hrec
