Automata/Util.lean
@@ -1,3 +1,0 @@
-theorem Vector.get_ofFn {α} {n: Nat} {f: Fin n → α} {i: Fin n}:
-    (Vector.ofFn f).get i = f i :=
-  Array.getElem_ofFn _
